
    \item ...\\
    \begin{eqnarray*} 
        \sigma_n &=& \sum_{i = 1}^n (x_i - \bar{x}_n)^2 \\
        &=& \sum_{i = 1}^{n - 1} (x_ i - \bar{x}_n)^2 + (x_n - \bar{x}_n)^2 \\
        &=& \sum_{i = 1}^{n - 1} \left( (x_i - \bar{x}_{n - 1}) - \frac{1}{n} (x_n - \bar{x}_{n - 1}) \right)^2 + \frac{(n - 1)^2}{n^2} (x_n - \bar{x}_{n - 1})^2 \\
        &=& \sum_{i = 1}^{n - 1} \left( (x_i - \bar{x}_{n - 1})^2 + \underbrace{\frac{1}{n^2}(x_n - \bar{x}_{n - 1})^2}_{\rightarrow (n - 1) \times â€¦} - \frac{2(x_n - \bar{x}_{n - 1})}{n} \underbrace{\sum_{i = 1}^{n - 1} (x_i - \bar{x}_{n - 1})}_{= 0}  \right) + \frac{(n - 1)^2}{n^2} (x_n - \bar{x}_{n - 1})^2 \\
        &=& \sum_{i = 1}^{n - 1} (x_i - \bar{x}_{n - 1})^2 + \underbrace{\left( \frac{n - 1}{n^2} + \frac{(n - 1)^2}{n^2}\right)}_{= \frac{(n - 1)}{n}} (x_n - \bar{x}_{n - 1})^2 \\
        &=&  \sigma_{n - 1} + \frac{(n - 1)}{n} (x_n - \bar{x}_{n - 1})^2.\\
    \end{eqnarray*} 
    \hfill$\square$